coq-minuska/theories/pval_ocaml_binding.v
@@ -4,27 +4,40 @@ From Minuska Require Import
     builtin.empty
     builtin.klike
     pi.trivial
+    hidden.hidden_unit
 .
 
 From Coq Require Import String ZArith.
 
 
-Record BuiltinInterface (NondetValue : Type) := mkBuiltinInterface {
+Record ValueAlgebraInterface (NondetValue : Type) := mkValueAlgebraInterface {
     bi_signature : Signature ;
     bi_beta : Model bi_signature NondetValue ;
     bi_sym_info : string -> SymbolInfo ;
 }.
 
-Definition builtins_empty : BuiltinInterface MyUnit := {|
+Record HiddenAlgebraInterface (NondetValue : Type)
+:= mkHiddenAlgebraInterface {
+    hai_vai : ValueAlgebraInterface NondetValue ;
+    hai_signature : HiddenSignature ;
+    hai_model : HiddenModel _ hai_signature hai_vai.(bi_beta _)  ;
+}.
+
+Definition builtins_empty : ValueAlgebraInterface MyUnit := {|
     bi_beta := builtin.empty.β ;
     bi_sym_info := fun s => si_none ;
 |}.
 
-Definition builtins_klike : BuiltinInterface MyUnit := {|
+Definition builtins_klike : ValueAlgebraInterface MyUnit := {|
     bi_beta := builtin.klike.β ;
     bi_sym_info := builtin.klike.sym_info ;
 |}.
 
 Definition pi_trivial := (@pi.trivial.MyProgramInfo string _ MyUnit, @pi.trivial.my_binding).
 
+Definition hai_klike : HiddenAlgebraInterface MyUnit := {|
+    hai_vai := builtins_klike ;
+    hai_signature := _ ;
+    hai_model := unit_hidden_model _ _ _;
+|}.
 
